Library/Verified/Random.java
@@ -1,5 +1,0 @@
-package Library.Verified;
-
-public class Random {
-  
-}
