Examples/Examples.dfy
@@ -1,0 +1,33 @@
+/*******************************************************************************
+*  Copyright by the contributors to the Dafny Project
+*  SPDX-License-Identifier: MIT
+*******************************************************************************/
+
+include "../Library/Random.dfy"
+
+module RandomExamples {
+  import opened DafnyLibraries
+
+  method Main() {
+    var r := new Random();
+
+    for i := 0 to 9 {
+      var b := r.Coin();
+      print b, "\n";
+    }
+
+    print "\n";
+
+    for i := 0 to 9 {
+      var u := r.Uniform(9);
+      print u, "\n";
+    }
+
+    print "\n";
+
+    for i := 0 to 9 {
+      var u := r.UniformInterval(3, 6);
+      print u, "\n";
+    }
+  }
+}
