Library/Random.dfy
@@ -1,0 +1,46 @@
+include "Model/RandomNumberGenerator.dfy"
+include "Model/Model.dfy"
+
+module {:extern "DafnyLibraries"} DafnyLibraries {
+  import opened RandomNumberGenerator
+  import Model
+
+  class {:extern} Random {
+    ghost var s: RNG
+
+    constructor {:extern} ()
+    
+    method {:extern} Coin() returns (b: bool)
+      ensures Model.Coin(old(s)) == (b, s)
+
+    method Uniform(n: nat) returns (u: nat)
+      requires n > 0
+      ensures Model.Uniform(n)(old(s)) == (u, s)
+    {
+      assume {:axiom} false;
+      var v := 1;
+      u := 0;
+      while true {
+        v := 2 * v;
+        var b := Coin();
+        u := 2 * u + if b then 1 else 0;
+        if v >= n {
+          if u < n {
+            return;
+          } else {
+            v := v - n;
+            u := u - n;
+          }
+        }
+      }
+    }
+    
+    method UniformInterval(a: int, b: int) returns (u: int)
+      requires a < b
+      ensures Model.UniformInterval(a, b)(old(s)) == (u, s)
+    {
+      var v := Uniform(b - a);
+      u := a + v;
+    }
+  }
+}
