README.md
@@ -4,14 +4,14 @@ The `Random` module introduces utils for probabilistic reasoning in Dafny. At th
 
 To use `Random` in your code, you must:
 
-1. `include` and `import` the `Random` module (either from `Verified/` or `Unverified/`) as you would any other library module
+1. `include` and `import` the `Random` module as you would any other library module
 2. incorporate the corresponding language-specific implementation file (that is, currently, `Random.java`) when building or running your program
 
-For example, to run the `RandomExamples.dfy` file in the `Examples` directory with the (unverified) `Random` module, run the following.
+For example, to run the `Examples.dfy` file in the `Examples` directory with the (unverified) `Random` module, run the following.
 
 ```bash
 # Java
-$ dafny run RandomExamples.dfy --target:java --input Unverified/Random.java
+$ dafny run Examples.dfy --target:java --input ./Library/Random.java
 ```
 
 (If you aren't using `dafny run` to run your program,
